[nameless] some substitution functions and equality lemma

coq/debruijn/Lambda.v
@@ -1,81 +1,124 @@
+Require Import Coq.Arith.Compare_dec Omega ssreflect.
 
-Require Import Arith.
-Require Import Coq.Arith.Compare_dec.
-Require Import Omega.
+Inductive term : Set := var of nat | app of term & term | abs of term.
 
-Inductive term : Type :=
-  | var : nat -> term
-  | app : term -> term -> term
-  | abs : term -> term.
-
-Inductive shifted1 : nat -> nat -> term -> Type :=
-  | svar1 : forall d c n, n < c -> shifted1 d c (var n)
-  | svar2 : forall d c n, c + d <= n -> d <= n -> shifted1 d c (var n)
-  | sapp : forall d c t1 t2, shifted1 d c t1 -> shifted1 d c t2 -> shifted1 d c (app t1 t2)
-  | sabs : forall d c t, shifted1 d (S c) t -> shifted1 d c (abs t).
-
-Fixpoint shift (d c : nat) (t : term) : term :=
+Fixpoint shift d c t : term :=
   match t with
-    | var n =>
-      match le_dec c n with
-        | left p => var (d + n)
-        | right p => var n
-      end
+    | var n => (if le_dec c n then var (n + d) else var n)%GEN_IF
     | app t1 t2 => app (shift d c t1) (shift d c t2)
     | abs t1 => abs (shift d (S c) t1)
   end.
 
-Functional Scheme shift_ind := Induction for shift Sort Prop.
-
-Definition shifted2 (d c : nat) (t : term) : Type :=
-  { t' : term | shift d c t' = t }.
-
-Lemma shifted1_shift : forall d c t, shifted1 d c (shift d c t).
-  intros.
-  revert d c.
-  induction t ; intros ; simpl.
-  case (le_dec c n) ; intros.
-  apply svar2 ; omega.
-  apply svar1 ; omega.
-  apply sapp ; auto.
-  apply sabs ; auto.
-Qed.
-
-Theorem shifted1_is_shifted2 : forall d c t, shifted1 d c t -> shifted2 d c t.
-  intros.
-  induction H.
-  exists (var n) ; simpl.
-  case (le_dec c n) ; intros.
-  apply False_ind ; omega.
-  auto.
-  exists (var (n - d)) ; simpl.
-  case (le_dec c (n - d)) ; intros.
-  f_equal ; omega.
-  apply False_ind ; omega.
-  elim IHshifted1_1 ; elim IHshifted1_2 ; intros.
-  exists (app x0 x) ; simpl.
-  f_equal ; auto.
-  elim IHshifted1 ; intros.
-  exists (abs x) ; simpl.
-  f_equal ; auto.
-Qed.
-
-Theorem shifted2_is_shifted1 : forall d c t, shifted2 d c t -> shifted1 d c t.
-  intros.
-  destruct X.
-  rewrite <- e.
-  exact (shifted1_shift d c x).
-Qed.
-
-Fixpoint unshift1 (d c : nat) (t : term) : term :=
+Fixpoint unshift d c t : term :=
   match t with
-    | var n =>
-      match le_dec c n with
-        | left p => var (n - d)
-        | right p => var n
-      end
-    | app t1 t2 => app (unshift1 d c t1) (unshift1 d c t2)
-    | abs t1 => abs (unshift1 d (S c) t1)
+    | var n => (if le_dec c n then var (n - d) else var n)%GEN_IF
+    | app t1 t2 => app (unshift d c t1) (unshift d c t2)
+    | abs t1 => abs (unshift d (S c) t1)
   end.
 
-Definition unshift2 (d c : nat) (t : term) (p : shifted2 d c t) : term := proj1_sig p.
+Fixpoint substitution1 t1 n t2 : term :=
+  match t2 with
+    | var m => (if eq_nat_dec n m then t1 else var m)%GEN_IF
+    | app t2l t2r => app (substitution1 t1 n t2l) (substitution1 t1 n t2r)
+    | abs t2' => abs (substitution1 (shift 1 0 t1) (S n) t2')
+  end.
+
+Fixpoint substitution2 s t1 n t2 : term :=
+  match t2 with
+    | var m => (if eq_nat_dec n m then shift s 0 t1 else var m)%GEN_IF
+    | app t2l t2r => app (substitution2 s t1 n t2l) (substitution2 s t1 n t2r)
+    | abs t2' => abs (substitution2 (S s) t1 (S n) t2')
+  end.
+
+Fixpoint substitution3 s t1 n t2 : term :=
+  match t2 with
+    | var m =>
+      match lt_eq_lt_dec n m with
+        | inleft (left p) => var (pred m)
+        | inleft (right p) => shift s 0 t1
+        | inright p => var m
+      end
+    | app t2l t2r => app (substitution3 s t1 n t2l) (substitution3 s t1 n t2r)
+    | abs t2' => abs (substitution3 (S s) t1 (S n) t2')
+  end.
+
+Lemma shift_add :
+  forall d d' c c' t, c <= c' <= d + c ->
+  shift d' c' (shift d c t) = shift (d' + d) c t.
+Proof.
+  move=> d d' c c' t; case; move: t c c'; elim.
+  - move=> n c c' H H0; simpl.
+    case le_dec => H1; simpl; case le_dec => H2; f_equal; omega.
+  - move=> t1 H t2 H0 c c' H1 H2; simpl; f_equal; auto.
+  - move=> t H c c' H0 H1; simpl; f_equal; apply H; omega.
+Qed.
+
+Lemma shiftzero_eq : forall n t, shift 0 n t = t.
+Proof.
+  move=> n t; move: t n; elim.
+  - move=> m n; simpl.
+    case le_dec => H; f_equal; omega.
+  - by move=> t1 H t2 H0 n; simpl; f_equal.
+  - move=> t H n; simpl; f_equal; apply H.
+Qed.
+
+Lemma unshift_shift_sub1 :
+  forall d d' c c' t, c <= c' <= d + c -> d' <= d ->
+  unshift d' c' (shift d c t) = shift (d - d') c t.
+Proof.
+  move=> d d' c c' t; case; move: t c c'; elim.
+  - move=> n c c' H H0 H1; simpl.
+    case le_dec=> H2; simpl; case le_dec=> H3; try omega; f_equal; omega.
+  - move=> t1 H t2 H0 c c' H1 H2 H3; simpl.
+    f_equal; auto.
+  - move=> t H c c' H0 H1 H2; simpl.
+    f_equal; apply H; omega.
+Qed.
+
+Lemma unshift_shift_eq :
+  forall d c c' t, c <= c' <= d + c -> unshift d c' (shift d c t) = t.
+Proof.
+  move=> d c c' t H.
+  rewrite unshift_shift_sub1; auto.
+  replace (d - d) with 0 by omega.
+  apply shiftzero_eq.
+Qed.
+
+Lemma substitution_eq_1_2 :
+  forall s t1 n t2, substitution1 (shift s 0 t1) n t2 = substitution2 s t1 n t2.
+Proof.
+  move=> s t1 n t2; move: t2 s t1 n; elim.
+  - move=> m s t1 n; simpl; by case eq_nat_dec=> H.
+  - move=> t2l H t2r H0 s t1 n; simpl; f_equal; auto.
+  - move=> t2' H s t1 n; simpl; f_equal; rewrite shift_add.
+    by replace (1 + s) with (S s) by omega.
+    omega.
+Qed.
+
+Lemma substitution_eq_2_3 :
+  forall t1 n t2,
+    unshift 1 n (substitution2 n (shift 1 0 t1) n t2) = substitution3 n t1 n t2.
+Proof.
+  move=> t1 n t2; move: t2 t1 n; elim.
+  - move=> m t1 n; simpl; case eq_nat_dec, lt_eq_lt_dec; try omega.
+    - case s=> H; try omega; clear.
+      rewrite shift_add; last omega.
+      replace (n + 1) with (S n) by omega.
+      rewrite unshift_shift_sub1; first f_equal; omega.
+    - case s=> H; try omega; simpl; case le_dec=> H0; f_equal; omega.
+    - simpl; case le_dec=> H; f_equal; omega.
+  - by move=> ? ? ? ? ? ?; simpl; f_equal.
+  - by move=> ? ? ? ?; simpl; f_equal.
+Qed.
+
+Lemma substitution_eq_1_3 :
+  forall t1 n t2,
+    unshift 1 n (substitution1 (shift (S n) 0 t1) n t2) =
+    substitution3 n t1 n t2.
+Proof.
+  move=> t1 n t2.
+  replace (S n) with (n + 1) by omega.
+  rewrite -(shift_add 1 n 0 0); last omega.
+  rewrite substitution_eq_1_2.
+  apply substitution_eq_2_3.
+Qed.
